$X^{out}_{RA} \leq B^{out}_{RA} * r$ \\
$Q^{out}_{RA} - X^{out}_{RA} \leq (1-B^{out}_{RA}) * r$ \\
$Q^{out}_{RA} \geq 0$ \\
$X^{in}_{RA} \leq B^{in}_{RA} * r$ \\
$Q^{in}_{RA} - X^{in}_{RA} \leq (1-B^{in}_{RA}) * r$ \\
$Q^{in}_{RA} \geq 0$ \\
$X^{outrRL}_{RA} \leq B^{outrRL}_{RA} * r$ \\
$Q^{outrRL}_{RA} - X^{outrRL}_{RA} \leq (1-B^{outrRL}_{RA}) * r$ \\
$Q^{outrRL}_{RA} \geq 0$ \\
$X^{inrRL}_{RA} \leq B^{inrRL}_{RA} * r$ \\
$Q^{inrRL}_{RA} - X^{inrRL}_{RA} \leq (1-B^{inrRL}_{RA}) * r$ \\
$Q^{inrRL}_{RA} \geq 0$ \\
$X^{outrDA}_{RA} \leq B^{outrDA}_{RA} * r$ \\
$Q^{outrDA}_{RA} - X^{outrDA}_{RA} \leq (1-B^{outrDA}_{RA}) * r$ \\
$Q^{outrDA}_{RA} \geq 0$ \\
$X^{inrDA}_{RA} \leq B^{inrDA}_{RA} * r$ \\
$Q^{inrDA}_{RA} - X^{inrDA}_{RA} \leq (1-B^{inrDA}_{RA}) * r$ \\
$Q^{inrDA}_{RA} \geq 0$ \\
$X^{outrRLDA}_{RA} \leq B^{outrRLDA}_{RA} * r$ \\
$Q^{outrRLDA}_{RA} - X^{outrRLDA}_{RA} \leq (1-B^{outrRLDA}_{RA}) * r$ \\
$Q^{outrRLDA}_{RA} \geq 0$ \\
$X^{inrRLDA}_{RA}  \leq B^{inrRLDA}_{RA} * r$ \\
$Q^{inrRLDA}_{RA}  - X^{inrRLDA}_{RA} \leq (1-B^{inrRLDA}_{RA}) * r$ \\
$Q^{inrRLDA}_{RA}  \geq 0$ \\



$X^{out}_{RL} \leq B^{out}_{RL} * r$ \\
$Q^{out}_{RL} - X^{out}_{RL} \leq (1-B^{out}_{RL}) * r$ \\
$Q^{out}_{RL} \geq 0$ \\
$X^{in}_{RL} \leq B^{in}_{RL} * r$ \\
$Q^{in}_{RL} - X^{in}_{RL} \leq (1-B^{in}_{RL}) * r$ \\
$Q^{in}_{RL} \geq 0$ \\
$X_{DA} \leq B_{DA} * r$ \\
$Q_{DA} - X_{DA} \leq (1-B_{DA}) * r$ \\
$Q_{DA} \geq 0$ \\


$c^{in}_{RL} \leq p(s^{in}_{RL}) + M * B^{in}_{RL}(s^{in}_{RL})\quad\forall s^{in}_{RL} $ \\
$c^{in}_{RL} \geq p(s^{in}_{RL}) - M * (1 - B^{in}_{RL}(s^{in}_{RL}))\quad\forall s^{in}_{RL} $ \\

$c^{out}_{RL} \leq p(s^{out}_{RL}) + M * B^{out}_{RL}(s^{out}_{RL})\quad\forall s^{out}_{RL} $ \\
$c^{out}_{RL} \geq p(s^{out}_{RL}) - M * (1 - B^{out}_{RL}(s^{out}_{RL}))\quad\forall s^{out}_{RL} $ \\

$c_{DA} \leq p(s_{DA}) + M * B_{DA}(s_{DA})\quad\forall s_{DA} $ \\
$c_{DA} \geq p(s_{DA}) - M * (1 - B_{DA}(s_{DA}))\quad\forall s_{DA} $ \\