$\sum_{s^{out}_{RA}} Q^{out}_{RA} \geq \sum_{s^{out}_{RL}} Q^{out}_{RL} $\\
$\sum_{s^{in}_{RA}} Q^{in}_{RA} \geq \sum_{s^{in}_{RL}} Q^{in}_{RL} $\\
$\sum_{s^{out}_{RA}} Q^{outrRL}_{RA} \geq \sum_{s^{out}_{RL}} Q^{out}_{RL} $\\
$\sum_{s^{in}_{RA}} Q^{inrRL}_{RA} \geq \sum_{s^{in}_{RL}} Q^{in}_{RL} $\\
$\sum_{s^{out}_{RA}} Q^{outrDA}_{RA} \geq \sum_{s^{out}_{RL}} Q^{out}_{RL} $\\
$\sum_{s^{in}_{RA}} Q^{inrDA}_{RA} \geq \sum_{s^{in}_{RL}} Q^{in}_{RL} $\\
$\sum_{s^{out}_{RA}} Q^{outrRLDA}_{RA} \geq \sum_{s^{out}_{RL}} Q^{out}_{RL} $\\
$\sum_{s^{in}_{RA}} Q^{inrRLDA}_{RA} \geq \sum_{s^{in}_{RL}} Q^{in}_{RL} $\\